Define tensor morphism
Not in the original posts but may be implicit or anyway useful.

cf6Script.sml
@@ -235,4 +235,129 @@ Proof
   \\ simp[Abbr`z`]
 QED
 
+Definition tensor_morphism_def:
+  tensor_morphism f c1 c2 g d1 d2 =
+    mk_chu_morphism (tensor c1 d1) (tensor c2 d2)
+      <| map_agent := λp. let (a,b) = decode_pair p in
+                            encode_pair (f.map.map_agent a, g.map.map_agent b);
+         map_env := λe. let m = decode_morphism c2 (swap d2) e in
+           encode_morphism
+             (mk_chu_morphism c1 (swap d1)
+               <| map_agent := g.map.map_env o m.map.map_agent o f.map.map_agent;
+                  map_env := f.map.map_env o m.map.map_env o g.map.map_agent |>) |>
+End
+
+Theorem tensor_morphism_maps_to:
+  f :- c1 → c2 -: chu w ∧
+  g :- d1 → d2 -: chu w
+  ⇒
+  tensor_morphism f c1 c2 g d1 d2 :- tensor c1 d1 → tensor c2 d2 -: chu w
+Proof
+  reverse(rw[maps_to_in_chu])
+  >- rw[tensor_morphism_def]
+  >- rw[tensor_morphism_def]
+  \\ `f.dom.world = w ∧ f.cod.world = w ∧ g.dom.world = w ∧ g.cod.world = w` by fs[chu_objects_def]
+  \\ simp[is_chu_morphism_def]
+  \\ conj_tac >- simp[tensor_morphism_def, mk_chu_morphism_def]
+  \\ conj_tac >- simp[tensor_morphism_def, mk_chu_morphism_def]
+  \\ conj_asm1_tac >- (
+    simp[tensor_morphism_def, mk_chu_morphism_def, restrict_def]
+    \\ simp[tensor_def, PULL_EXISTS, hom_def]
+    \\ gen_tac \\ strip_tac
+    \\ qmatch_goalsub_abbrev_tac`encode_morphism m`
+    \\ qexists_tac`m` \\ simp[]
+    \\ simp[maps_to_in_chu]
+    \\ simp[Abbr`m`]
+    \\ DEP_REWRITE_TAC[decode_encode_chu_morphism]
+    \\ simp[is_chu_morphism_def]
+    \\ simp[extensional_def]
+    \\ fs[is_chu_morphism_def, maps_to_in_chu] )
+  \\ conj_asm1_tac >- (
+    simp[tensor_morphism_def, mk_chu_morphism_def, restrict_def]
+    \\ simp[tensor_def, PULL_EXISTS, EXISTS_PROD]
+    \\ fs[is_chu_morphism_def] )
+  \\ qx_genl_tac[`a`,`e`]
+  \\ strip_tac
+  \\ first_x_assum drule
+  \\ first_x_assum drule
+  \\ ntac 2 (pop_assum mp_tac)
+  \\ simp[tensor_def, mk_cf_def, hom_def, PULL_EXISTS, EXISTS_PROD]
+  \\ rpt strip_tac
+  \\ reverse IF_CASES_TAC >- metis_tac[]
+  \\ pop_assum kall_tac
+  \\ DEP_REWRITE_TAC[decode_encode_chu_morphism] \\ simp[]
+  \\ qmatch_rename_tac`f.dom.eval a1 (m2.map.map_env a2) =
+                       f.cod.eval b1 (m1.map.map_env b2)`
+  \\ qpat_x_assum`_ = encode_pair _`mp_tac
+  \\ qpat_x_assum`_ = encode_morphism _`mp_tac
+  \\ simp[tensor_morphism_def, mk_chu_morphism_def, tensor_def, restrict_def, hom_def]
+  \\ reverse IF_CASES_TAC >- metis_tac[]
+  \\ pop_assum kall_tac
+  \\ qmatch_goalsub_abbrev_tac`encode_morphism m3`
+  \\ strip_tac
+  \\ `decode_morphism f.dom (swap g.dom) (encode_morphism m3) =
+      decode_morphism f.dom (swap g.dom) (encode_morphism m2)` by metis_tac[]
+  \\ pop_assum mp_tac
+  \\ DEP_REWRITE_TAC[decode_encode_chu_morphism] \\ simp[]
+  \\ conj_tac >- (
+    simp[maps_to_in_chu]
+    \\ simp[Abbr`m3`]
+    \\ simp[is_chu_morphism_def]
+    \\ simp[extensional_def]
+    \\ DEP_REWRITE_TAC[decode_encode_chu_morphism] \\ simp[]
+    \\ pop_assum kall_tac
+    \\ fs[maps_to_in_chu, is_chu_morphism_def])
+  \\ disch_then(strip_assume_tac o SYM)
+  \\ disch_then(strip_assume_tac o GSYM)
+  \\ fs[maps_to_in_chu, is_chu_morphism_def]
+  \\ simp[Abbr`m3`]
+  \\ DEP_REWRITE_TAC[decode_encode_chu_morphism] \\ simp[]
+  \\ fs[maps_to_in_chu, is_chu_morphism_def]
+QED
+
+(*
+Theorem iso_tensor:
+  c1 ≅ c2 -: chu w ∧ d1 ≅ d2 -: chu w ⇒
+  tensor c1 d1 ≅ tensor c2 d2 -: chu w
+Proof
+  simp[iso_objs_thm, GSYM AND_IMP_INTRO]
+  \\ disch_then(qx_choose_then`f`strip_assume_tac)
+  \\ disch_then(qx_choose_then`g`strip_assume_tac)
+  \\ qexists_tac`tensor_morphism f c1 c2 g d1 d2`
+  \\ conj_asm1_tac >- simp[tensor_morphism_maps_to]
+  \\ fs[chu_iso_bij]
+  \\ simp[Once CONJ_ASSOC]
+  \\ reverse conj_tac >- fs[maps_to_in_chu]
+QED
+
+Theorem tensor_assoc:
+  c1 ∈ chu_objects w ∧ c2 ∈ chu_objects w ∧ c3 ∈ chu_objects w ⇒
+  tensor c1 (tensor c2 c3) ≅ tensor (tensor c1 c2) c3 -: chu w
+Proof
+  `∀c1 c2 c3.
+    c1 ∈ chu_objects w ∧ c2 ∈ chu_objects w ∧ c3 ∈ chu_objects w ⇒
+    tensor (tensor c1 c2) c3 ≅ tensor (tensor c1 c3) c2 -: chu w`
+  suffices_by (
+    rpt strip_tac
+    \\ irule iso_objs_trans \\ simp[]
+    \\ qexists_tac`tensor c1 (tensor c3 c2)`
+    \\ conj_tac >- ( irule iso_tensor \\ simp[] \\ irule tensor_comm \\ simp[] )
+    \\ irule iso_objs_trans \\ simp[]
+    \\ qexists_tac`tensor (tensor c3 c2) c1`
+    \\ conj_tac >- metis_tac[tensor_comm, tensor_in_chu_objects]
+    \\ irule iso_objs_trans \\ simp[]
+    \\ qexists_tac`tensor (tensor c3 c1) c2`
+    \\ conj_tac >- metis_tac[]
+    \\ irule iso_objs_trans \\ simp[]
+    \\ qexists_tac`tensor (tensor c1 c3) c2`
+    \\ conj_tac >- ( irule iso_tensor \\ simp[] \\ irule tensor_comm \\ simp[] )
+    \\ metis_tac[] )
+  \\
+
+Theorem homotopy_equiv_tensor_right:
+  c1 ∈ chu_objects w ∧ c2 ∈ chu_objects w ∧ d ∈ chu_objects w ∧
+  c1 ≃ c2 -: w ⇒
+  tensor c1 d ≃ tensor c2 d -: w
+*)
+
 val _ = export_theory();
